ACL2Lean/Imported/SimpleWorld.lean
@@ -1,0 +1,29 @@
+import ACL2Lean.Eval
+
+open ACL2
+
+namespace ACL2.Worlds.Simple
+
+private def sym (name : String) : Symbol := ⟨"ACL2", name⟩
+
+def my_lenBody : SExpr :=
+  (SExpr.cons (SExpr.atom (.symbol { name := "if" })) (SExpr.cons (SExpr.cons (SExpr.atom (.symbol { name := "consp" })) (SExpr.cons (SExpr.atom (.symbol { name := "x" })) SExpr.nil)) (SExpr.cons (SExpr.cons (SExpr.atom (.symbol { name := "+" })) (SExpr.cons (SExpr.atom (.number (.int (1)))) (SExpr.cons (SExpr.cons (SExpr.atom (.symbol { name := "my-len" })) (SExpr.cons (SExpr.cons (SExpr.atom (.symbol { name := "cdr" })) (SExpr.cons (SExpr.atom (.symbol { name := "x" })) SExpr.nil)) SExpr.nil)) SExpr.nil))) (SExpr.cons (SExpr.atom (.number (.int (0)))) SExpr.nil))))
+
+def my_appBody : SExpr :=
+  (SExpr.cons (SExpr.atom (.symbol { name := "if" })) (SExpr.cons (SExpr.cons (SExpr.atom (.symbol { name := "consp" })) (SExpr.cons (SExpr.atom (.symbol { name := "x" })) SExpr.nil)) (SExpr.cons (SExpr.cons (SExpr.atom (.symbol { name := "cons" })) (SExpr.cons (SExpr.cons (SExpr.atom (.symbol { name := "car" })) (SExpr.cons (SExpr.atom (.symbol { name := "x" })) SExpr.nil)) (SExpr.cons (SExpr.cons (SExpr.atom (.symbol { name := "my-app" })) (SExpr.cons (SExpr.cons (SExpr.atom (.symbol { name := "cdr" })) (SExpr.cons (SExpr.atom (.symbol { name := "x" })) SExpr.nil)) (SExpr.cons (SExpr.atom (.symbol { name := "y" })) SExpr.nil))) SExpr.nil))) (SExpr.cons (SExpr.atom (.symbol { name := "y" })) SExpr.nil))))
+
+def world : World where
+  defs := ({} : Std.HashMap Symbol (List Symbol × SExpr))
+    |>.insert (sym "my-len") ([sym "x"], my_lenBody)
+    |>.insert (sym "my-app") ([sym "x", sym "y"], my_appBody)
+
+def defaultFuel : Nat := 1000000
+
+def my_len_my_appFormula : SExpr :=
+  (SExpr.cons (SExpr.atom (.symbol { name := "equal" })) (SExpr.cons (SExpr.cons (SExpr.atom (.symbol { name := "my-len" })) (SExpr.cons (SExpr.cons (SExpr.atom (.symbol { name := "my-app" })) (SExpr.cons (SExpr.atom (.symbol { name := "x" })) (SExpr.cons (SExpr.atom (.symbol { name := "y" })) SExpr.nil))) SExpr.nil)) (SExpr.cons (SExpr.cons (SExpr.atom (.symbol { name := "+" })) (SExpr.cons (SExpr.cons (SExpr.atom (.symbol { name := "my-len" })) (SExpr.cons (SExpr.atom (.symbol { name := "x" })) SExpr.nil)) (SExpr.cons (SExpr.cons (SExpr.atom (.symbol { name := "my-len" })) (SExpr.cons (SExpr.atom (.symbol { name := "y" })) SExpr.nil)) SExpr.nil))) SExpr.nil)))
+
+theorem my_len_my_app (env : Env) :
+    eval defaultFuel world env my_len_my_appFormula = SExpr.t := sorry
+
+end ACL2.Worlds.Simple
+
